compiler/backend/proofs/stack_allocProofScript.sml
@@ -3596,19 +3596,38 @@ val word_gen_gc_partial_move_roots_bitmaps_code_thm =
   \\ once_rewrite_tac [split_num_forall_to_10]
   \\ full_simp_tac(srw_ss())[nine_less] \\ fs []);
 
+val word_gen_gc_move_list_code_def = Define `
+  word_gen_gc_move_list_code conf =
+    While NotEqual 7 (Imm (0w:'a word))
+      (list_Seq [load_inst 5 8;
+                 sub_1_inst 7;
+                 word_gen_gc_move_code conf;
+                 store_inst 5 8;
+                 add_bytes_in_word_inst 8])`
 
-
-(*
+val word_gen_gc_partial_move_list_code_def = Define `
+  word_gen_gc_partial_move_list_code conf =
+    While NotEqual 7 (Imm (0w:'a word))
+      (list_Seq [load_inst 5 8;
+                 sub_1_inst 7;
+                 word_gen_gc_partial_move_code conf;
+                 store_inst 5 8;
+                 add_bytes_in_word_inst 8])`
 
 val word_gen_gc_move_list_code_thm = Q.store_thm("word_gen_gc_move_list_code_thm",
-  `!l a (s:('a,'b)stackSem$state) pa1 pa old m1 m i1 i dm conf a1.
-      word_gen_gc_move_list conf (a:'a word,l,i,pa,old,m,dm) = (a1,i1,pa1,m1,T) /\
+  `!l a (s:('a,'b)stackSem$state) pa1 pa old m1 m i1 i dm conf a1 ib ib1 pb pb1.
+      word_gen_gc_move_list conf (a:'a word,l,i,pa,ib,pb,old,m,dm) =
+         (a1,i1,pa1,ib1,pb1,m1,T) /\
       shift_length conf < dimindex (:'a) /\ word_shift (:'a) < dimindex (:'a) /\
       2 < dimindex (:'a) /\ conf.len_size <> 0 /\
       (!w:'a word. w << word_shift (:'a) = w * bytes_in_word) /\
       FLOOKUP s.store CurrHeap = SOME (Word old) /\ s.use_store /\
       s.memory = m /\ s.mdomain = dm /\
-       0 IN FDOM s.regs /\
+      Temp 0w IN FDOM s.store /\
+      Temp 1w IN FDOM s.store /\
+      FLOOKUP s.store (Temp 2w) = SOME (Word pb) /\
+      FLOOKUP s.store (Temp 3w) = SOME (Word ib) /\
+      0 IN FDOM s.regs /\
       1 IN FDOM s.regs /\
       2 IN FDOM s.regs /\
       get_var 3 s = SOME (Word pa) /\
@@ -3617,9 +3636,13 @@ val word_gen_gc_move_list_code_thm = Q.store_thm("word_gen_gc_move_list_code_thm
       6 IN FDOM s.regs ==>
       get_var 7 s = SOME (Word l) /\
       get_var 8 s = SOME (Word a) ==>
-      ?ck r0 r1 r2 r5 r6.
+      ?ck r0 r1 r2 r5 r6 t0 t1.
         evaluate (word_gen_gc_move_list_code conf,s with clock := s.clock + ck) =
           (NONE,s with <| memory := m1;
+                          store :=
+                            s.store |++
+                            [(Temp 0w,t0); (Temp 1w,t1); (Temp 2w,Word pb1);
+                             (Temp 3w,Word ib1)];
                           regs := s.regs |++ [(0,r0);
                                               (1,r1);
                                               (2,r2);
@@ -3637,10 +3660,13 @@ val word_gen_gc_move_list_code_thm = Q.store_thm("word_gen_gc_move_list_code_thm
     \\ full_simp_tac(srw_ss())[FUPDATE_LIST,GSYM fmap_EQ,FLOOKUP_DEF,EXTENSION,
            FUN_EQ_THM,FAPPLY_FUPDATE_THM]
     \\ once_rewrite_tac [split_num_forall_to_10]
-    \\ full_simp_tac(srw_ss())[nine_less])
+    \\ full_simp_tac(srw_ss())[nine_less]
+    \\ qexists_tac `s.store ' (Temp 0w)`
+    \\ qexists_tac `s.store ' (Temp 1w)`
+    \\ rw [] \\ eq_tac \\ rw[] \\ fs [])
   \\ once_rewrite_tac [word_gen_gc_move_list_def] \\ simp [LET_THM]
   \\ rpt strip_tac \\ simp [LET_THM]
-  \\ qpat_x_assum `_ = (a1,i1,pa1,m1,T)` mp_tac
+  \\ qpat_x_assum `_ = (a1,i1,pa1,ib1,pb1,m1,T)` mp_tac
   \\ `n2w (SUC n) + -1w = n2w n` by fs [ADD1,GSYM word_add_n2w]
   \\ pairarg_tac \\ simp []
   \\ pairarg_tac \\ simp []
@@ -3655,6 +3681,99 @@ val word_gen_gc_move_list_code_thm = Q.store_thm("word_gen_gc_move_list_code_thm
   \\ fs [GSYM word_gen_gc_move_list_code_def,get_var_def,get_var_imm_def]
   \\ tac
   \\ drule (word_gen_gc_move_code_thm |> GEN_ALL)
+  \\ fs [ADD1,GSYM word_add_n2w]
+  \\ `FLOOKUP ((s:('a,'b)stackSem$state) with
+           <|regs := s.regs |+ (5,s.memory a) |+ (7,Word (n2w n)) |>).store
+       CurrHeap  = SOME (Word old)` by fs []
+  \\ disch_then drule \\ fs [get_var_def] \\ tac \\ strip_tac
+  \\ fs []
+  \\ first_x_assum (qspec_then `s with
+        <|regs :=
+            s.regs |+ (5,s.memory a) |+ (7,Word (n2w n)) |+ (0,r0) |+
+            (1,r1) |+ (2,r2) |+ (3,Word pa1') |+ (4,Word i1') |+
+            (5,w1) |+ (6,r6) |+ (8,Word (a + bytes_in_word));
+          store :=
+            s.store |+ (Temp 0w,t0) |+ (Temp 1w,t1) |+
+            (Temp 2w,Word pb') |+ (Temp 3w,Word ib');
+          memory := (a =+ w1) m1' |>` mp_tac)
+  \\ rpt (impl_tac THEN1 (fs [] \\ tac)) \\ fs []
+  \\ strip_tac \\ fs []
+  \\ qexists_tac `ck+ck'+1` \\ fs []
+  \\ pop_assum mp_tac
+  \\ drule (evaluate_add_clock |> GEN_ALL)
+  \\ disch_then (qspec_then `ck'+1` strip_assume_tac)
+  \\ fs [AC ADD_COMM ADD_ASSOC] \\ tac
+  \\ strip_tac
+  \\ drule (evaluate_add_clock |> GEN_ALL)
+  \\ disch_then (qspec_then `ck` strip_assume_tac)
+  \\ fs [AC ADD_COMM ADD_ASSOC] \\ tac
+  \\ fs [STOP_def]
+  \\ full_simp_tac(srw_ss())[state_component_equality]
+  \\ full_simp_tac(srw_ss())[FUPDATE_LIST,GSYM fmap_EQ,FLOOKUP_DEF,EXTENSION,
+         FUN_EQ_THM,FAPPLY_FUPDATE_THM]
+  \\ once_rewrite_tac [split_num_forall_to_10]
+  \\ full_simp_tac(srw_ss())[nine_less]
+  \\ qexists_tac `t0'` \\ qexists_tac `t1'`
+  \\ rw [] \\ eq_tac \\ rw [] \\ fs []);
+
+val word_gen_gc_partial_move_list_code_thm = Q.store_thm("word_gen_gc_partial_move_list_code_thm",
+  `!l a (s:('a,'b)stackSem$state) pa1 pa old m1 m i1 i dm conf a1 gs rs.
+      word_gen_gc_partial_move_list conf (a:'a word,l,i,pa,old,m,dm,gs,rs) =
+         (a1,i1,pa1,m1,T) /\
+      shift_length conf < dimindex (:'a) /\ word_shift (:'a) < dimindex (:'a) /\
+      2 < dimindex (:'a) /\ conf.len_size <> 0 /\
+      (!w:'a word. w << word_shift (:'a) = w * bytes_in_word) /\
+      FLOOKUP s.store CurrHeap = SOME (Word old) /\ s.use_store /\
+      s.memory = m /\ s.mdomain = dm /\ good_dimindex (:'a) /\
+      FLOOKUP s.store (Temp 0w) = SOME (Word gs) /\
+      FLOOKUP s.store (Temp 1w) = SOME (Word rs) /\
+      0 IN FDOM s.regs /\
+      1 IN FDOM s.regs /\
+      2 IN FDOM s.regs /\
+      get_var 3 s = SOME (Word pa) /\
+      get_var 4 s = SOME (Word (i:'a word)) /\
+      5 IN FDOM s.regs ==>
+      6 IN FDOM s.regs ==>
+      get_var 7 s = SOME (Word l) /\
+      get_var 8 s = SOME (Word a) ==>
+      ?ck r0 r1 r2 r5 r6.
+        evaluate (word_gen_gc_partial_move_list_code conf,s with clock := s.clock + ck) =
+          (NONE,s with <| memory := m1;
+                          regs := s.regs |++ [(0,r0);
+                                              (1,r1);
+                                              (2,r2);
+                                              (3,Word pa1);
+                                              (4,Word i1);
+                                              (5,r5);
+                                              (6,r6);
+                                              (7,Word 0w);
+                                              (8,Word a1)] |>)`,
+  Cases \\ Induct_on `n` \\ simp [] THEN1
+   (fs [Once word_gen_gc_partial_move_list_def] \\ rw []
+    \\ qexists_tac `0`
+    \\ fs [word_gen_gc_partial_move_list_code_def,get_var_def] \\ tac
+    \\ full_simp_tac(srw_ss())[state_component_equality]
+    \\ full_simp_tac(srw_ss())[FUPDATE_LIST,GSYM fmap_EQ,FLOOKUP_DEF,EXTENSION,
+           FUN_EQ_THM,FAPPLY_FUPDATE_THM]
+    \\ once_rewrite_tac [split_num_forall_to_10]
+    \\ full_simp_tac(srw_ss())[nine_less])
+  \\ once_rewrite_tac [word_gen_gc_partial_move_list_def] \\ simp [LET_THM]
+  \\ rpt strip_tac \\ simp [LET_THM]
+  \\ qpat_x_assum `_ = (a1,i1,pa1,m1,T)` mp_tac
+  \\ `n2w (SUC n) + -1w = n2w n` by fs [ADD1,GSYM word_add_n2w]
+  \\ pairarg_tac \\ simp []
+  \\ pairarg_tac \\ simp []
+  \\ strip_tac
+  \\ rpt var_eq_tac
+  \\ `n < dimword (:'a)` by decide_tac
+  \\ first_x_assum drule
+  \\ disch_then drule
+  \\ fs [] \\ strip_tac
+  \\ rpt var_eq_tac \\ fs []
+  \\ simp [word_gen_gc_partial_move_list_code_def,evaluate_def]
+  \\ fs [GSYM word_gen_gc_partial_move_list_code_def,get_var_def,get_var_imm_def]
+  \\ tac
+  \\ drule (word_gen_gc_partial_move_code_thm |> GEN_ALL)
   \\ fs [ADD1,GSYM word_add_n2w]
   \\ `FLOOKUP ((s:('a,'b)stackSem$state) with
            <|regs := s.regs |+ (5,s.memory a) |+ (7,Word (n2w n)) |>).store
@@ -3683,17 +3802,48 @@ val word_gen_gc_move_list_code_thm = Q.store_thm("word_gen_gc_move_list_code_thm
   \\ full_simp_tac(srw_ss())[FUPDATE_LIST,GSYM fmap_EQ,FLOOKUP_DEF,EXTENSION,
          FUN_EQ_THM,FAPPLY_FUPDATE_THM]
   \\ once_rewrite_tac [split_num_forall_to_10]
-  \\ full_simp_tac(srw_ss())[nine_less])
+  \\ full_simp_tac(srw_ss())[nine_less]);
 
-val word_gen_gc_move_loop_code_thm = Q.prove(
-  `!k pb1 i1 pa1 old1 m1 dm1 c1 i2 pa2 m2 (s:('a,'b)stackSem$state).
-      word_gen_gc_move_loop k conf (pb1,i1,pa1,old1,m1,dm1,c1) = (i2,pa2,m2,T) /\
+val word_gen_gc_move_data_code_def = Define `
+  word_gen_gc_move_data_code conf =
+    While NotEqual 3 (Reg 8)
+     (list_Seq [load_inst 7 8;
+                If Test 7 (Imm 4w)
+                  (list_Seq [right_shift_inst 7 (dimindex (:α) - conf.len_size);
+                             add_bytes_in_word_inst 8;
+                             word_gen_gc_move_list_code conf])
+                  (list_Seq [right_shift_inst 7 (dimindex (:α) - conf.len_size);
+                             add_1_inst 7;
+                             left_shift_inst 7 (word_shift (:'a));
+                             add_inst 8 7])]):'a stackLang$prog`
+
+val word_gen_gc_partial_move_data_code_def = Define `
+  word_gen_gc_partial_move_data_code conf =
+    While NotEqual 3 (Reg 8)
+     (list_Seq [load_inst 7 8;
+                If Test 7 (Imm 4w)
+                  (list_Seq [right_shift_inst 7 (dimindex (:α) - conf.len_size);
+                             add_bytes_in_word_inst 8;
+                             word_gen_gc_partial_move_list_code conf])
+                  (list_Seq [right_shift_inst 7 (dimindex (:α) - conf.len_size);
+                             add_1_inst 7;
+                             left_shift_inst 7 (word_shift (:'a));
+                             add_inst 8 7])]):'a stackLang$prog`
+
+val word_gen_gc_move_data_code_thm = Q.prove(
+  `!k ha1 i1 pa1 ib1 pb1 old1 m1 dm1 c1 i2 pa2 ib2 pb2 m2 (s:('a,'b)stackSem$state).
+      word_gen_gc_move_data conf k (ha1,i1,pa1,ib1,pb1,old1,m1,dm1) =
+        (i2,pa2,ib2,pb2,m2,T) /\
       shift_length conf < dimindex (:'a) /\ word_shift (:'a) < dimindex (:'a) /\
       2 < dimindex (:'a) /\ conf.len_size <> 0 /\
       conf.len_size + 2 < dimindex (:'a) /\
       (!w:'a word. w << word_shift (:'a) = w * bytes_in_word) /\
       FLOOKUP s.store CurrHeap = SOME (Word old1) /\ s.use_store /\
       s.memory = m1 /\ s.mdomain = dm1 /\
+      Temp 0w IN FDOM s.store /\
+      Temp 1w IN FDOM s.store /\
+      FLOOKUP s.store (Temp 2w) = SOME (Word pb1) /\
+      FLOOKUP s.store (Temp 3w) = SOME (Word ib1) /\
       0 IN FDOM s.regs /\
       1 IN FDOM s.regs /\
       2 IN FDOM s.regs /\
@@ -3702,9 +3852,137 @@ val word_gen_gc_move_loop_code_thm = Q.prove(
       5 IN FDOM s.regs ==>
       6 IN FDOM s.regs ==>
       7 IN FDOM s.regs ==>
-      get_var 8 s = SOME (Word pb1) /\ c1 ==>
-      ?ck r0 r1 r2 r5 r6 r7.
-        evaluate (word_gen_gc_move_loop_code conf,s with clock := s.clock + ck) =
+      get_var 8 s = SOME (Word ha1) /\ c1 ==>
+      ?ck r0 r1 r2 r5 r6 r7 t0 t1.
+        evaluate (word_gen_gc_move_data_code conf,s with clock := s.clock + ck) =
+          (NONE,s with <| memory := m2;
+                          store :=
+                            s.store |++
+                            [(Temp 0w,t0); (Temp 1w,t1); (Temp 2w,Word pb2);
+                             (Temp 3w,Word ib2)];
+                          regs := s.regs |++ [(0,r0);
+                                              (1,r1);
+                                              (2,r2);
+                                              (3,Word pa2);
+                                              (4,Word i2);
+                                              (5,r5);
+                                              (6,r6);
+                                              (7,r7);
+                                              (8,Word pa2)] |>)`,
+  strip_tac \\ completeInduct_on `k` \\ rpt strip_tac
+  \\ qpat_x_assum `word_gen_gc_move_data _ _ _ = _` mp_tac
+  \\ once_rewrite_tac [word_gen_gc_move_data_def]
+  \\ IF_CASES_TAC THEN1
+   (fs [] \\ rw [] \\ fs [] \\ rpt var_eq_tac
+    \\ fs [word_gen_gc_move_data_code_def,get_var_def] \\ tac
+    \\ full_simp_tac(srw_ss())[state_component_equality]
+    \\ full_simp_tac(srw_ss())[FUPDATE_LIST,GSYM fmap_EQ,FLOOKUP_DEF,EXTENSION,
+           FUN_EQ_THM,FAPPLY_FUPDATE_THM]
+    \\ once_rewrite_tac [split_num_forall_to_10]
+    \\ full_simp_tac(srw_ss())[nine_less]
+    \\ qexists_tac `s.store ' (Temp 0w)`
+    \\ qexists_tac `s.store ' (Temp 1w)`
+    \\ rw [] \\ eq_tac \\ rw[] \\ fs [])
+  \\ IF_CASES_TAC \\ fs []
+  \\ `k-1 < k` by decide_tac
+  \\ first_x_assum drule \\ ntac 2 (pop_assum kall_tac) \\ strip_tac
+  \\ rpt var_eq_tac \\ fs []
+  \\ pairarg_tac \\ fs []
+  \\ Cases_on `word_bit 2 (theWord (s.memory ha1))`
+  \\ fs [word_bit_test] THEN1
+   (rpt strip_tac \\ fs [] \\ fs [] \\ rveq
+    \\ asm_simp_tac std_ss[word_gen_gc_move_data_code_def,evaluate_def]
+    \\ asm_simp_tac std_ss[GSYM word_gen_gc_move_data_code_def,STOP_def]
+    \\ fs [get_var_def,isWord_thm,clear_top_inst_def] \\ tac
+    \\ rev_full_simp_tac(srw_ss())
+         [data_to_wordPropsTheory.decode_length_def,LET_THM] \\ rpt var_eq_tac
+    \\ full_simp_tac(srw_ss())[theWord_def] \\ tac
+    \\ rev_full_simp_tac(srw_ss())[select_lower_lemma,
+         DECIDE ``n<>0 ==> m-(n-1)-1=m-n:num``,theWord_def]
+    \\ qabbrev_tac `ww = bytes_in_word *
+          (v ⋙ (dimindex (:α) − conf.len_size) + 1w)`
+    \\ qabbrev_tac `s5 = s with
+        <|regs := s.regs |+ (7,Word v) |+
+                            (7,Word ww) |+ (8,Word (ha1 + ww)) |>`
+    \\ `s.memory = s5.memory /\ s.mdomain = s5.mdomain` by
+         (unabbrev_all_tac \\ fs [])
+    \\ fs [] \\ first_x_assum drule \\ fs []
+    \\ fs [AND_IMP_INTRO] \\ impl_tac
+    THEN1 (unabbrev_all_tac \\ fs [FLOOKUP_UPDATE])
+    \\ strip_tac \\ qexists_tac `ck + 1` \\ fs []
+    \\ qunabbrev_tac `s5` \\ fs []
+    \\ full_simp_tac(srw_ss())[state_component_equality]
+    \\ full_simp_tac(srw_ss())[FUPDATE_LIST,GSYM fmap_EQ,FLOOKUP_DEF,EXTENSION,
+           FUN_EQ_THM,FAPPLY_FUPDATE_THM]
+    \\ once_rewrite_tac [split_num_forall_to_10]
+    \\ full_simp_tac(srw_ss())[nine_less]
+    \\ qexists_tac `t0` \\ qexists_tac `t1`
+    \\ rw [] \\ eq_tac \\ rw[] \\ fs [])
+  \\ rpt strip_tac
+  \\ asm_simp_tac std_ss[word_gen_gc_move_data_code_def,evaluate_def]
+  \\ asm_simp_tac std_ss[GSYM word_gen_gc_move_data_code_def,STOP_def]
+  \\ rev_full_simp_tac(srw_ss())[] \\ rpt var_eq_tac
+  \\ fs [get_var_def,isWord_thm,clear_top_inst_def] \\ tac
+  \\ full_simp_tac(srw_ss())[theWord_def] \\ tac
+  \\ rev_full_simp_tac(srw_ss())[select_lower_lemma,
+       DECIDE ``n<>0 ==> m-(n-1)-1=m-n:num``,theWord_def]
+  \\ rev_full_simp_tac(srw_ss())
+         [data_to_wordPropsTheory.decode_length_def,LET_THM] \\ rpt var_eq_tac
+  \\ rpt (pairarg_tac \\ fs []) \\ rveq \\ fs [] \\ tac
+  \\ qabbrev_tac `s5 = s with
+        <|regs :=
+            s.regs |+ (7,Word v) |+
+            (7,Word (v ⋙ (dimindex (:'a) − conf.len_size))) |+
+            (8,Word (ha1 + bytes_in_word)) |>`
+  \\ drule word_gen_gc_move_list_code_thm
+  \\ disch_then (qspec_then `s5` mp_tac)
+  \\ fs [AND_IMP_INTRO] \\ impl_tac
+  THEN1 (unabbrev_all_tac \\ fs [FLOOKUP_UPDATE,get_var_def,theWord_def])
+  \\ strip_tac \\ fs [GSYM CONJ_ASSOC]
+  \\ pop_assum mp_tac
+  \\ qpat_abbrev_tac `s6 = s5 with <|regs := _ ; store := _ ; memory := _ |>`
+  \\ `s.mdomain = s6.mdomain /\ m'' = s6.memory` by (unabbrev_all_tac \\ fs [])
+  \\ qpat_x_assum `Abbrev _` assume_tac
+  \\ fs [] \\ qpat_x_assum `_ = _` kall_tac
+  \\ first_x_assum drule \\ impl_tac
+  THEN1 (unabbrev_all_tac \\ fs [FUPDATE_LIST,FLOOKUP_UPDATE])
+  \\ rpt strip_tac \\ qexists_tac `ck + ck' + 1`
+  \\ drule (evaluate_add_clock |> GEN_ALL)
+  \\ disch_then (qspec_then `ck'+1` mp_tac) \\ fs []
+  \\ qunabbrev_tac `s5` \\ fs [] \\ strip_tac
+  \\ qunabbrev_tac `s6`
+  \\ fs [theWord_def]
+  \\ full_simp_tac(srw_ss())[state_component_equality]
+  \\ full_simp_tac(srw_ss())[FUPDATE_LIST,GSYM fmap_EQ,FLOOKUP_DEF,EXTENSION,
+         FUN_EQ_THM,FAPPLY_FUPDATE_THM]
+  \\ once_rewrite_tac [split_num_forall_to_10]
+  \\ full_simp_tac(srw_ss())[nine_less]
+  \\ qexists_tac `t0'` \\ qexists_tac `t1'`
+  \\ rw [] \\ eq_tac \\ rw[] \\ fs []);
+
+val word_gen_gc_partial_move_data_code_thm = Q.prove(
+  `!k ha1 i1 pa1 old1 m1 dm1 c1 i2 pa2 m2 (s:('a,'b)stackSem$state).
+      word_gen_gc_partial_move_data conf k (ha1,i1,pa1,old1,m1,dm1,gs,rs) =
+        (i2,pa2,m2,T) /\
+      shift_length conf < dimindex (:'a) /\ word_shift (:'a) < dimindex (:'a) /\
+      2 < dimindex (:'a) /\ conf.len_size <> 0 /\
+      conf.len_size + 2 < dimindex (:'a) /\
+      (!w:'a word. w << word_shift (:'a) = w * bytes_in_word) /\
+      FLOOKUP s.store CurrHeap = SOME (Word old1) /\ s.use_store /\
+      s.memory = m1 /\ s.mdomain = dm1 /\ good_dimindex (:'a) /\
+      FLOOKUP s.store (Temp 0w) = SOME (Word gs) /\
+      FLOOKUP s.store (Temp 1w) = SOME (Word rs) /\
+      0 IN FDOM s.regs /\
+      1 IN FDOM s.regs /\
+      2 IN FDOM s.regs /\
+      get_var 3 s = SOME (Word pa1) /\
+      get_var 4 s = SOME (Word (i1:'a word)) /\
+      5 IN FDOM s.regs ==>
+      6 IN FDOM s.regs ==>
+      7 IN FDOM s.regs ==>
+      get_var 8 s = SOME (Word ha1) /\ c1 ==>
+      ?ck r0 r1 r2 r5 r6 r7 t0 t1.
+        evaluate (word_gen_gc_partial_move_data_code conf,s with clock := s.clock + ck) =
           (NONE,s with <| memory := m2;
                           regs := s.regs |++ [(0,r0);
                                               (1,r1);
@@ -3716,11 +3994,11 @@ val word_gen_gc_move_loop_code_thm = Q.prove(
                                               (7,r7);
                                               (8,Word pa2)] |>)`,
   strip_tac \\ completeInduct_on `k` \\ rpt strip_tac
-  \\ qpat_x_assum `word_gen_gc_move_loop _ _ _ = _` mp_tac
-  \\ once_rewrite_tac [word_gen_gc_move_loop_def]
+  \\ qpat_x_assum `word_gen_gc_partial_move_data _ _ _ = _` mp_tac
+  \\ once_rewrite_tac [word_gen_gc_partial_move_data_def]
   \\ IF_CASES_TAC THEN1
    (fs [] \\ rw [] \\ fs [] \\ rpt var_eq_tac
-    \\ fs [word_gen_gc_move_loop_code_def,get_var_def] \\ tac
+    \\ fs [word_gen_gc_partial_move_data_code_def,get_var_def] \\ tac
     \\ full_simp_tac(srw_ss())[state_component_equality]
     \\ full_simp_tac(srw_ss())[FUPDATE_LIST,GSYM fmap_EQ,FLOOKUP_DEF,EXTENSION,
            FUN_EQ_THM,FAPPLY_FUPDATE_THM]
@@ -3731,12 +4009,11 @@ val word_gen_gc_move_loop_code_thm = Q.prove(
   \\ first_x_assum drule \\ ntac 2 (pop_assum kall_tac) \\ strip_tac
   \\ rpt var_eq_tac \\ fs []
   \\ pairarg_tac \\ fs []
-  \\ Cases_on `word_bit 2 (theWord (s.memory pb1))`
+  \\ Cases_on `word_bit 2 (theWord (s.memory ha1))`
   \\ fs [word_bit_test] THEN1
-   (strip_tac
-    \\ drule word_gen_gc_move_loop_ok \\ fs [] \\ strip_tac \\ fs []
-    \\ asm_simp_tac std_ss[word_gen_gc_move_loop_code_def,evaluate_def]
-    \\ asm_simp_tac std_ss[GSYM word_gen_gc_move_loop_code_def,STOP_def]
+   (rpt strip_tac \\ fs [] \\ fs [] \\ rveq
+    \\ asm_simp_tac std_ss[word_gen_gc_partial_move_data_code_def,evaluate_def]
+    \\ asm_simp_tac std_ss[GSYM word_gen_gc_partial_move_data_code_def,STOP_def]
     \\ fs [get_var_def,isWord_thm,clear_top_inst_def] \\ tac
     \\ rev_full_simp_tac(srw_ss())
          [data_to_wordPropsTheory.decode_length_def,LET_THM] \\ rpt var_eq_tac
@@ -3747,7 +4024,7 @@ val word_gen_gc_move_loop_code_thm = Q.prove(
           (v ⋙ (dimindex (:α) − conf.len_size) + 1w)`
     \\ qabbrev_tac `s5 = s with
         <|regs := s.regs |+ (7,Word v) |+
-                            (7,Word ww) |+ (8,Word (pb1 + ww)) |>`
+                            (7,Word ww) |+ (8,Word (ha1 + ww)) |>`
     \\ `s.memory = s5.memory /\ s.mdomain = s5.mdomain` by
          (unabbrev_all_tac \\ fs [])
     \\ fs [] \\ first_x_assum drule \\ fs []
@@ -3760,10 +4037,9 @@ val word_gen_gc_move_loop_code_thm = Q.prove(
            FUN_EQ_THM,FAPPLY_FUPDATE_THM]
     \\ once_rewrite_tac [split_num_forall_to_10]
     \\ full_simp_tac(srw_ss())[nine_less])
-  \\ strip_tac
-  \\ drule word_gen_gc_move_loop_ok \\ fs [] \\ strip_tac \\ fs []
-  \\ asm_simp_tac std_ss[word_gen_gc_move_loop_code_def,evaluate_def]
-  \\ asm_simp_tac std_ss[GSYM word_gen_gc_move_loop_code_def,STOP_def]
+  \\ rpt strip_tac
+  \\ asm_simp_tac std_ss[word_gen_gc_partial_move_data_code_def,evaluate_def]
+  \\ asm_simp_tac std_ss[GSYM word_gen_gc_partial_move_data_code_def,STOP_def]
   \\ rev_full_simp_tac(srw_ss())[] \\ rpt var_eq_tac
   \\ fs [get_var_def,isWord_thm,clear_top_inst_def] \\ tac
   \\ full_simp_tac(srw_ss())[theWord_def] \\ tac
@@ -3771,19 +4047,20 @@ val word_gen_gc_move_loop_code_thm = Q.prove(
        DECIDE ``n<>0 ==> m-(n-1)-1=m-n:num``,theWord_def]
   \\ rev_full_simp_tac(srw_ss())
          [data_to_wordPropsTheory.decode_length_def,LET_THM] \\ rpt var_eq_tac
+  \\ rpt (pairarg_tac \\ fs []) \\ rveq \\ fs [] \\ tac
   \\ qabbrev_tac `s5 = s with
         <|regs :=
             s.regs |+ (7,Word v) |+
             (7,Word (v ⋙ (dimindex (:'a) − conf.len_size))) |+
-            (8,Word (pb1 + bytes_in_word)) |>`
-  \\ drule word_gen_gc_move_list_code_thm
+            (8,Word (ha1 + bytes_in_word)) |>`
+  \\ drule word_gen_gc_partial_move_list_code_thm
   \\ disch_then (qspec_then `s5` mp_tac)
   \\ fs [AND_IMP_INTRO] \\ impl_tac
-  THEN1 (unabbrev_all_tac \\ fs [FLOOKUP_UPDATE,get_var_def])
+  THEN1 (unabbrev_all_tac \\ fs [FLOOKUP_UPDATE,get_var_def,theWord_def])
   \\ strip_tac \\ fs [GSYM CONJ_ASSOC]
   \\ pop_assum mp_tac
   \\ qpat_abbrev_tac `s6 = s5 with <|regs := _ ; memory := _ |>`
-  \\ `s.mdomain = s6.mdomain /\ m1 = s6.memory` by (unabbrev_all_tac \\ fs [])
+  \\ `s.mdomain = s6.mdomain /\ m'' = s6.memory` by (unabbrev_all_tac \\ fs [])
   \\ qpat_x_assum `Abbrev _` assume_tac
   \\ fs [] \\ qpat_x_assum `_ = _` kall_tac
   \\ first_x_assum drule \\ impl_tac
@@ -3793,11 +4070,17 @@ val word_gen_gc_move_loop_code_thm = Q.prove(
   \\ disch_then (qspec_then `ck'+1` mp_tac) \\ fs []
   \\ qunabbrev_tac `s5` \\ fs [] \\ strip_tac
   \\ qunabbrev_tac `s6`
+  \\ fs [theWord_def]
   \\ full_simp_tac(srw_ss())[state_component_equality]
   \\ full_simp_tac(srw_ss())[FUPDATE_LIST,GSYM fmap_EQ,FLOOKUP_DEF,EXTENSION,
          FUN_EQ_THM,FAPPLY_FUPDATE_THM]
   \\ once_rewrite_tac [split_num_forall_to_10]
   \\ full_simp_tac(srw_ss())[nine_less]);
+
+(*
+
+word_gen_gc_move_refs_def
+word_gen_gc_move_loop_def
 
 *)
 
